progress on basic properties of logical relation

theories/LogicalRelation.v
@@ -3,7 +3,7 @@
 From Stdlib Require Import Utf8 List Arith Bool Lia Wellfounded.Inverse_Image Wellfounded.Inclusion.
 From TypedConfluence.autosubst
 Require Import core unscoped AST SubstNotations RAsimpl AST_rasimpl.
-From TypedConfluence Require Import Util BasicAST Weakenings Contexts Typing BasicMetaTheory. (*  Env Inst. *)
+From TypedConfluence Require Import Util BasicAST Weakenings Contexts Typing BasicMetaTheory Reduction. (*  Env Inst. *)
 From Stdlib Require Import Setoid Morphisms Relation_Definitions.
 Require Import Stdlib.Program.Equality.
 Import CombineNotations.
@@ -67,7 +67,7 @@ Definition LogRel := term -> term -> TmRel -> Prop.
 Definition LRΩ : LogRel := fun A B R => ∙ ⊢< Ax prop > A ≡ B : Sort prop /\ forall t u : term, R t u <-> ∙ ⊢< prop > t ≡ u : A.
 
 Definition ϵNat : TmRel := 
-    fun t1 t2 => exists k, ∙ ⊢< ty 0 > t1 ≡ (mk_Nat k) : Nat /\ ∙ ⊢< ty 0 > t2 ≡ (mk_Nat k) : Nat.
+    fun t1 t2 => exists k, ∙ ⊢< ty 0 > t1 -->>! (mk_Nat k) : Nat /\ ∙ ⊢< ty 0 > t2 -->>! (mk_Nat k) : Nat.
 
 Definition ϵPi i j S1 S2 (ϵS : TmRel) T1 T2 (ϵT : forall s1 s2, ϵS s1 s2 -> TmRel) : TmRel 
     := fun f1 f2 => 
@@ -75,44 +75,59 @@ Definition ϵPi i j S1 S2 (ϵS : TmRel) T1 T2 (ϵT : forall s1 s2, ϵS s1 s2 -> 
         forall s1 s2 (ϵs : ϵS s1 s2), ϵT s1 s2 ϵs (app i j S1 T1 f1 s1) (app i j S2 T2 f2 s2).
 
 (* TODO replace conv by reduction *)
+
+
+Notation "R1 <~> R2" :=  (forall t u, R1 t u <-> R2 t u) (at level 50, R2 at next level).
+
 Inductive LRTy : forall (k : nat) (rec : forall j, j ◃ (ty k) -> LogRel), LogRel :=
-| LRTy_nat A1 A2 rec : 
-    ∙ ⊢< Ax (ty 0) > A1 ≡ Nat : Sort (ty 0) -> 
-    ∙ ⊢< Ax (ty 0) > A2 ≡ Nat : Sort (ty 0) ->
-    LRTy 0 rec A1 A2 ϵNat
-| LRTy_pi1 i k A1 A2 S1 S2 ϵS T1 T2 ϵT
+| LRTy_nat A1 A2 rec R : 
+    ∙ ⊢< Ax (ty 0) > A1 -->>! Nat : Sort (ty 0) -> 
+    ∙ ⊢< Ax (ty 0) > A2 -->>! Nat : Sort (ty 0) ->
+    R <~> ϵNat ->
+    LRTy 0 rec A1 A2 R
+| LRTy_pi1 i k A1 A2 S1 S2 ϵS T1 T2 ϵT R
     (rec : forall j, j ◃ ty k -> LogRel)
     (q : i ◃ ty k) :
-    ∙ ⊢< Ax (Ru i (ty k)) > A1 ≡ Pi i (ty k) S1 T1 : Sort (Ru i (ty k)) -> 
-    ∙ ⊢< Ax (Ru i (ty k)) > A2 ≡ Pi i (ty k) S2 T2 : Sort (Ru i (ty k)) ->
-    ∙ ⊢< Ax (Ru i (ty k)) > A1 ≡ A2 : Sort (Ru i (ty k)) ->
+    ∙ ⊢< Ax (Ru i (ty k)) > A1 -->>! Pi i (ty k) S1 T1 : Sort (Ru i (ty k)) -> 
+    ∙ ⊢< Ax (Ru i (ty k)) > A2 -->>! Pi i (ty k) S2 T2 : Sort (Ru i (ty k)) ->
+    (* ∙ ⊢< Ax (Ru i (ty k)) > A1 ≡ A2 : Sort (Ru i (ty k)) -> *)
+    ∙ ⊢< Ax i > S1 ≡ S2 : Sort i -> 
+    ∙ ,, (i, S1) ⊢< Ax (ty k) > T1 ≡ T2 : Sort (ty k) ->
     rec i q S1 S2 ϵS ->
     (forall s1 s2 (ϵs : ϵS s1 s2), 
-        LRTy k rec T1 T2 (ϵT s1 s2 ϵs)) ->
-    LRTy k rec A1 A2 (ϵPi i (ty k) S1 S2 ϵS T1 T2 ϵT)
-| LRTy_pi2 k A1 A2 S1 S2 ϵS T1 T2 ϵT
+        LRTy k rec (T1 <[ s1 ..]) (T2 <[ s2 ..]) (ϵT s1 s2 ϵs)) ->
+    R <~> (ϵPi i (ty k) S1 S2 ϵS T1 T2 ϵT) ->
+    LRTy k rec A1 A2 R
+| LRTy_pi2 k A1 A2 S1 S2 ϵS T1 T2 ϵT R
     (rec : forall j, j ◃ ty k -> LogRel) :
-    ∙ ⊢< Ax (Ru (ty k) (ty k)) > A1 ≡ Pi (ty k) (ty k) S1 T1 : Sort (Ru (ty k) (ty k)) -> 
-    ∙ ⊢< Ax (Ru (ty k) (ty k)) > A2 ≡ Pi (ty k) (ty k) S2 T2 : Sort (Ru (ty k) (ty k)) ->
-    ∙ ⊢< Ax (Ru (ty k) (ty k)) > A1 ≡ A2 : Sort (Ru (ty k) (ty k)) ->
+    ∙ ⊢< Ax (Ru (ty k) (ty k)) > A1 -->>! Pi (ty k) (ty k) S1 T1 : Sort (Ru (ty k) (ty k)) -> 
+    ∙ ⊢< Ax (Ru (ty k) (ty k)) > A2 -->>! Pi (ty k) (ty k) S2 T2 : Sort (Ru (ty k) (ty k)) ->
+    (* ∙ ⊢< Ax (Ru (ty k) (ty k)) > A1 ≡ A2 : Sort (Ru (ty k) (ty k)) -> *)
+    ∙ ⊢< Ax (ty k) > S1 ≡ S2 : Sort (ty k) -> 
+    ∙ ,, (ty k, S1) ⊢< Ax (ty k) > T1 ≡ T2 : Sort (ty k) ->
     LRTy k rec S1 S2 ϵS ->
     (forall s1 s2 (ϵs : ϵS s1 s2), 
-        LRTy k rec T1 T2 (ϵT s1 s2 ϵs)) ->
-    LRTy k rec A1 A2 (ϵPi (ty k) (ty k) S1 S2 ϵS T1 T2 ϵT)
-| LRTy_pi3 n k A1 A2 S1 S2 ϵS T1 T2 ϵT
+        LRTy k rec (T1 <[ s1 ..]) (T2 <[ s2 ..]) (ϵT s1 s2 ϵs)) ->
+    R <~> (ϵPi (ty k) (ty k) S1 S2 ϵS T1 T2 ϵT) ->
+    LRTy k rec A1 A2 R
+| LRTy_pi3 n k A1 A2 S1 S2 ϵS T1 T2 ϵT R
     (rec : forall j, j ◃ ty n -> LogRel)
     (q : k < n) :
-    ∙ ⊢< Ax (Ru (ty n) (ty k)) > A1 ≡ Pi (ty n) (ty k) S1 T1 : Sort (Ru (ty n) (ty k)) -> 
-    ∙ ⊢< Ax (Ru (ty n) (ty k)) > A2 ≡ Pi (ty n) (ty k) S2 T2 : Sort (Ru (ty n) (ty k)) ->
-    ∙ ⊢< Ax (Ru (ty n) (ty k)) > A1 ≡ A2 : Sort (Ru (ty n) (ty k)) ->
+    ∙ ⊢< Ax (Ru (ty n) (ty k)) > A1 -->>! Pi (ty n) (ty k) S1 T1 : Sort (Ru (ty n) (ty k)) -> 
+    ∙ ⊢< Ax (Ru (ty n) (ty k)) > A2 -->>! Pi (ty n) (ty k) S2 T2 : Sort (Ru (ty n) (ty k)) ->
+    (* ∙ ⊢< Ax (Ru (ty n) (ty k)) > A1 ≡ A2 : Sort (Ru (ty n) (ty k)) -> *)
+    ∙ ⊢< Ax (ty n) > S1 ≡ S2 : Sort (ty n) -> 
+    ∙ ,, (ty n, S1) ⊢< Ax (ty k) > T1 ≡ T2 : Sort (ty k) ->
     LRTy n rec S1 S2 ϵS ->
     (forall s1 s2 (ϵs : ϵS s1 s2), 
-        rec (ty k) (ltac :(simpl; lia)) T1 T2 (ϵT s1 s2 ϵs)) ->
-    LRTy n rec A1 A2 (ϵPi (ty n) (ty k) S1 S2 ϵS T1 T2 ϵT)
-| LRTy_U l A1 A2 rec : 
-    ∙ ⊢< Ax (Ax l) > A1 ≡ Sort l : Sort (Ax l) -> 
-    ∙ ⊢< Ax (Ax l) > A2 ≡ Sort l : Sort (Ax l) ->
-    LRTy (ax l) rec A1 A2 (fun B1 B2 => exists R, rec l lt_ty_ax B1 B2 R).
+        rec (ty k) (ltac :(simpl; lia)) (T1 <[ s1 ..]) (T2 <[ s2 ..]) (ϵT s1 s2 ϵs)) ->
+    R <~> (ϵPi (ty n) (ty k) S1 S2 ϵS T1 T2 ϵT) ->
+    LRTy n rec A1 A2 R
+| LRTy_U l A1 A2 rec R : 
+    ∙ ⊢< Ax (Ax l) > A1 -->>! Sort l : Sort (Ax l) -> 
+    ∙ ⊢< Ax (Ax l) > A2 -->>! Sort l : Sort (Ax l) ->
+    R <~> (fun B1 B2 => exists R, rec l lt_ty_ax B1 B2 R) ->
+    LRTy (ax l) rec A1 A2 R.
 
 
 Definition LR (l : level) : LogRel.
@@ -122,6 +137,9 @@ Definition LR (l : level) : LogRel.
         + apply LRΩ.
     - apply wf_inverse_image. apply lt_wf.
 Defined.
+
+
+Notation "⊩< l > A ≡ B ↓ R" :=  (LR l A B R) (at level 50, A, B, R at next level).
 
 Axiom proof_irrel : forall (P : Prop) (p q : P), p = q.
 
@@ -166,73 +184,81 @@ end H) _ (F l p))).
     erewrite (@acc_irrel i (fun l _ => wf_inverse_image level nat lt lvl_to_nat lt_wf l)). reflexivity. reflexivity.
 Qed.
 
-Definition LR_nat A1 A2 : 
-    ∙ ⊢< Ax (ty 0) > A1 ≡ Nat : Sort (ty 0) -> 
-    ∙ ⊢< Ax (ty 0) > A2 ≡ Nat : Sort (ty 0) ->
-    LR (ty 0) A1 A2 ϵNat.
+Definition LR_nat A1 A2 R : 
+    ∙ ⊢< Ax (ty 0) > A1 -->>! Nat : Sort (ty 0) -> 
+    ∙ ⊢< Ax (ty 0) > A2 -->>! Nat : Sort (ty 0) ->
+    R <~> ϵNat ->
+    LR (ty 0) A1 A2 R.
 Proof.
     intros. rewrite LR_ty_eq.
     constructor; eauto.
 Qed.
 
-Definition LR_U l A1 A2 : 
-    ∙ ⊢< Ax (Ax l) > A1 ≡ Sort l : Sort (Ax l) -> 
-    ∙ ⊢< Ax (Ax l) > A2 ≡ Sort l : Sort (Ax l) ->
-    LR (Ax l) A1 A2 (fun B1 B2 => exists R, LR l B1 B2 R).
+Definition LR_U l A1 A2 R : 
+    ∙ ⊢< Ax (Ax l) > A1 -->>! Sort l : Sort (Ax l) -> 
+    ∙ ⊢< Ax (Ax l) > A2 -->>! Sort l : Sort (Ax l) ->
+    R <~> (fun B1 B2 => exists R, LR l B1 B2 R) ->
+    LR (Ax l) A1 A2 R.
 Proof.
     intros. unfold Ax. rewrite LR_ty_eq.
     constructor; eauto.
 Qed.
 
 
-Definition LR_pi i k A1 A2 S1 S2 ϵS T1 T2 ϵT : 
-    ∙ ⊢< Ax (Ru i (ty k)) > A1 ≡ Pi i (ty k) S1 T1 : Sort (Ru i (ty k)) -> 
-    ∙ ⊢< Ax (Ru i (ty k)) > A2 ≡ Pi i (ty k) S2 T2 : Sort (Ru i (ty k)) ->
-    ∙ ⊢< Ax (Ru i (ty k)) > A1 ≡ A2 : Sort (Ru i (ty k)) ->
+Definition LR_pi i k A1 A2 S1 S2 ϵS T1 T2 ϵT R : 
+    ∙ ⊢< Ax (Ru i (ty k)) > A1 -->>! Pi i (ty k) S1 T1 : Sort (Ru i (ty k)) -> 
+    ∙ ⊢< Ax (Ru i (ty k)) > A2 -->>! Pi i (ty k) S2 T2 : Sort (Ru i (ty k)) ->
+    ∙ ⊢< Ax i > S1 ≡ S2 : Sort i -> 
+    ∙ ,, (i, S1) ⊢< Ax (ty k) > T1 ≡ T2 : Sort (ty k) ->
     LR i S1 S2 ϵS -> 
-    (forall s1 s2 (ϵs : ϵS s1 s2), LR (ty k) T1 T2 (ϵT s1 s2 ϵs)) ->
-    LR (Ru i (ty k)) A1 A2 (ϵPi i (ty k) S1 S2 ϵS T1 T2 ϵT).
+    (forall s1 s2 (ϵs : ϵS s1 s2), LR (ty k) (T1 <[ s1 ..]) (T2 <[ s2 ..]) (ϵT s1 s2 ϵs)) ->
+    R <~> (ϵPi i (ty k) S1 S2 ϵS T1 T2 ϵT) ->
+    LR (Ru i (ty k)) A1 A2 R.
 Proof.
     intros. unfold Ru. rewrite LR_ty_eq.
     assert (i ⊴ (ty k) \/ ty k ◃ i) by eauto using Nat.le_gt_cases.
-    destruct H4. inversion H4.
-    - pose proof (f_equal nat_to_lvl H6) as H'. rewrite lvl_to_nat_to_lvl in H'. rewrite H' in *. 
-      simpl. assert (max k k = k) by lia. rewrite H5. apply LRTy_pi2; eauto. 
+    destruct H6. inversion H6.
+    - pose proof (f_equal nat_to_lvl H8) as H'. rewrite lvl_to_nat_to_lvl in H'. rewrite H' in *. 
+      simpl. assert (max k k = k) by lia. rewrite H7. eapply LRTy_pi2; eauto. 
       rewrite <- LR_ty_eq. auto.
       rewrite <- LR_ty_eq. auto.
-    - assert (ru i k = k). unfold ru. destruct i. simpl in H6. lia. auto.
-      rewrite H7. apply LRTy_pi1; auto. 
+    - assert (ru i k = k). unfold ru. destruct i. simpl in H8. lia. auto.
+      rewrite H9. eapply LRTy_pi1; eauto. 
       simpl. lia.
       rewrite <- LR_ty_eq. auto.
-    - destruct i. 2:inversion H4.
-      simpl in H4. assert (ru (ty n) k = n). unfold ru. lia.
-      rewrite H5. apply LRTy_pi3; auto. lia. 
-      rewrite <- LR_ty_eq. auto.
+    - destruct i. 2:inversion H6.
+      simpl in H6. assert (ru (ty n) k = n). unfold ru. lia.
+      rewrite H7. eapply LRTy_pi3; eauto. lia. 
+      rewrite <- LR_ty_eq. eauto.
 Qed.
 
 
 Definition LR_ind 
     (P : forall l A B R, Prop)
     (p_prop : forall A B R (p : LRΩ A B R), P prop A B R) 
-    (p_nat : forall A1 A2
-        (A1_red_nat : ∙ ⊢< Ax (ty 0) > A1 ≡ Nat : Sort (ty 0))
-        (A2_red_nat : ∙ ⊢< Ax (ty 0) > A2 ≡ Nat : Sort (ty 0)),
-        P (ty 0) A1 A2 ϵNat)
-    (p_U : forall l A1 A2
-        (A1_red_U : ∙ ⊢< Ax (Ax l) > A1 ≡ Sort l : Sort (Ax l))
-        (A2_red_U : ∙ ⊢< Ax (Ax l) > A2 ≡ Sort l : Sort (Ax l)),
+    (p_nat : forall A1 A2 R
+        (A1_red_nat : ∙ ⊢< Ax (ty 0) > A1 -->>! Nat : Sort (ty 0))
+        (A2_red_nat : ∙ ⊢< Ax (ty 0) > A2 -->>! Nat : Sort (ty 0)),
+        R <~> ϵNat ->
+        P (ty 0) A1 A2 R)
+    (p_U : forall l A1 A2 R
+        (A1_red_U : ∙ ⊢< Ax (Ax l) > A1 -->>! Sort l : Sort (Ax l))
+        (A2_red_U : ∙ ⊢< Ax (Ax l) > A2 -->>! Sort l : Sort (Ax l)),
         (forall B1 B2 R, LR l B1 B2 R -> P l B1 B2 R) ->
-        P (Ax l) A1 A2 (fun B1 B2 => exists R, LR l B1 B2 R))
-    (p_pi : forall i k A1 A2 S1 S2 ϵS T1 T2 ϵT
-        (A1_red_pi : ∙ ⊢< Ax (Ru i (ty k)) > A1 ≡ Pi i (ty k) S1 T1 : Sort (Ru i (ty k)))
-        (A2_red_pi : ∙ ⊢< Ax (Ru i (ty k)) > A2 ≡ Pi i (ty k) S2 T2 : Sort (Ru i (ty k)))
-        (A1_eq_A2 : ∙ ⊢< Ax (Ru i (ty k)) > A1 ≡ A2 : Sort (Ru i (ty k)))      
+        R <~> (fun B1 B2 => exists R, LR l B1 B2 R) ->
+        P (Ax l) A1 A2 R)
+    (p_pi : forall i k A1 A2 S1 S2 ϵS T1 T2 ϵT R
+        (A1_red_pi : ∙ ⊢< Ax (Ru i (ty k)) > A1 -->>! Pi i (ty k) S1 T1 : Sort (Ru i (ty k)))
+        (A2_red_pi : ∙ ⊢< Ax (Ru i (ty k)) > A2 -->>! Pi i (ty k) S2 T2 : Sort (Ru i (ty k)))
+        (S1_eq_S2 : ∙ ⊢< Ax i > S1 ≡ S2 : Sort i) 
+        (T1_eq_T2 : ∙ ,, (i, S1) ⊢< Ax (ty k) > T1 ≡ T2 : Sort (ty k))
         (LR_S : LR i S1 S2 ϵS)
         (LR_T : forall s1 s2 (ϵs : ϵS s1 s2), 
-                LR (ty k) T1 T2 (ϵT s1 s2 ϵs)),
+                LR (ty k) (T1 <[ s1 ..]) (T2 <[ s2 ..]) (ϵT s1 s2 ϵs)),
+        R <~> (ϵPi i (ty k) S1 S2 ϵS T1 T2 ϵT) ->
         P i S1 S2 ϵS -> 
-        (forall s1 s2 (ϵs : ϵS s1 s2), P (ty k) T1 T2 (ϵT s1 s2 ϵs)) ->
-        P (Ru i (ty k)) A1 A2 (ϵPi i (ty k) S1 S2 ϵS T1 T2 ϵT))
+        (forall s1 s2 (ϵs : ϵS s1 s2), P (ty k) (T1 <[ s1 ..]) (T2 <[ s2 ..]) (ϵT s1 s2 ϵs)) ->
+        P (Ru i (ty k)) A1 A2 R)
     (l : level) (A B : term) (R : TmRel) (x : LR l A B R) : P l A B R.
 Proof.
     generalize l A B R x.
@@ -247,18 +273,18 @@ Proof.
         rewrite <- H0 in x.
         induction x.
         + apply p_nat; auto.
-        + rewrite H0 in H4. rewrite H0 in H5. rewrite <- LR_ty_eq in H5.
+        + rewrite H0 in H5. rewrite H0 in H6. rewrite <- LR_ty_eq in H6.
           assert (k = ru i k). unfold ru. destruct i. simpl in q. lia. lia.
-          rewrite H7 at 1. apply p_pi; auto.
-        + rewrite H0 in H4. rewrite <- LR_ty_eq in H4.
+          rewrite H9 at 1. eapply p_pi; eauto.
+        + rewrite H0 in H5. rewrite <- LR_ty_eq in H5.
           rewrite H0 in x. rewrite <- LR_ty_eq in x.
           assert (k = ru (ty k) k). simpl. lia.
-          rewrite H6 at 1. apply p_pi; auto.
+          rewrite H8 at 1. eapply p_pi; eauto.
         + rewrite H0 in *. rewrite <- LR_ty_eq in x.
-          assert (ty n = Ru (ty n) (ty k)). simpl. f_equal. lia. rewrite H5 at 1.
-          apply p_pi; auto. 
+          assert (ty n = Ru (ty n) (ty k)). simpl. f_equal. lia. rewrite H7 at 1.
+          eapply p_pi; eauto. 
           intros. apply H. simpl. lia. auto.
-        + rewrite H0. apply p_U; auto.
+        + rewrite H0 in H3. eapply p_U; eauto.
     - rewrite LR_prop_eq in x. apply p_prop. auto.
 Qed.
 
@@ -269,50 +295,311 @@ Proof.
     refine (LR_ind _ _ _ _ _).
     - intros. split.
       + destruct p. auto.
-      + destruct p. intros. destruct (H0 t u). auto.
+      + destruct p. intros. eapply H0. eauto.
     - intros. split.
-      + eauto using conv_trans, conv_sym.
-      + intros. unfold ϵNat in H. destruct H as (k & H1 & H2). eauto using conv_trans, conv_sym, conv_conv.
+      + eauto using redd_whnf_to_conv, conv_trans, conv_sym.
+      + intros. unfold ϵNat in H. apply H in H0 as (k & H1 & H2). eauto 8 using redd_whnf_to_conv, conv_trans, conv_sym, conv_conv.
     - intros. split.
-      + eauto using conv_trans, conv_sym.
-      + intros. destruct H0 as (R & lr). apply H in lr as (t_eq_u & _). eauto using conv_trans, conv_sym, conv_conv.
+      + eauto using redd_whnf_to_conv, conv_trans, conv_sym.
+      + intros. apply H0 in H1 as (R' & lr). apply H in lr as (t_eq_u & _). eauto 8 using redd_whnf_to_conv, conv_trans, conv_sym, conv_conv.
     - intros. split; auto.
-      intros. destruct H1 as (H' & _). eauto using conv_conv, conv_sym.
+      intros. eapply redd_whnf_to_conv in A1_red_pi, A2_red_pi.
+      eapply conv_trans. eapply A1_red_pi. eapply conv_trans. 2:(eapply conv_sym; eapply A2_red_pi).
+      eapply conv_pi; eauto.
+      intros. rewrite H in H2. destruct H2. eauto using conv_conv, redd_whnf_to_conv, conv_sym.
 Qed.
 
-Lemma LR_sym l A B R : 
+Lemma LR_erasure l A B R : 
     LR l A B R -> 
-    LR l B A R /\ (forall t u, R t u -> R u t).
+    (forall A' B', 
+        ∙ ⊢< Ax l > A ~ A' : Sort l ->
+        ∙ ⊢< Ax l > B ~ B' : Sort l ->
+        LR l A' B' R) 
+    /\
+    (forall t u t' u', 
+        ∙ ⊢< l > t ~ t' : A -> 
+        ∙ ⊢< l > u ~ u' : A -> 
+        R t u -> 
+        R t' u').
 Proof.
     generalize l A B R. clear l A B R.
     refine (LR_ind _ _ _ _ _).
-    - intros. destruct p. split.
-        + rewrite LR_prop_eq. constructor. auto using conv_sym. intros. 
-          split; intro; destruct (H0 t u); eauto using conv_conv, conv_sym.
-        + intros. destruct (H0 u t). destruct (H0 t u). eauto using conv_conv, conv_sym.
-    - intros. split.
-        + apply LR_nat; auto.
-        + intros. destruct H as (k & H1 & H2). exists k. auto.
-    - intros. split.
-        + apply LR_U; auto.
-        + intros B1 B2 H0. destruct H0 as (R & lr). exists R. 
-          destruct (H B1 B2 R lr) as (H1 & H2). auto.
-    - intros. split.
-        + apply LR_pi; eauto using conv_sym, conv_trans.
-        + intros f1 f2 ϵf. split.
-            ++ destruct ϵf; eauto using conv_sym.
-            ++ intros. destruct ϵf.
-               destruct H as (LR_S' & sym_ϵS).
-               destruct (H0 s1 s2 ϵs) as (LR_T' & sym_ϵT).
-               admit. (* we need to be able to exchange converitble annotations *)
+    - intros. destruct p. split; intros.
+        + rewrite LR_prop_eq. split.
+            ++ eauto 6 using conv_sym, conv_trans, sim_to_conv.
+            ++ intros. destruct (H0 t u). split; eauto using conv_conv, conv_sym, sim_to_conv.
+        + destruct (H0 t' u'). destruct (H0 t u). eauto 8 using sim_to_conv, conv_trans, conv_sym.
+    - intros. split; intros.
+        + eapply sim_left_redd_whnf in A1_red_nat as (_Nat & A'_redd_nat & nat_sim); eauto.
+          eapply aconv_inv in nat_sim. simpl in nat_sim. subst.
+          eapply sim_left_redd_whnf in A2_red_nat as (_Nat & B'_redd_nat & nat_sim); eauto.
+          eapply aconv_inv in nat_sim. simpl in nat_sim. subst.
+          apply LR_nat; eauto.
+        + rewrite H in *. destruct H2 as (k & t_redd_k & u_redd_k).
+          unfold ϵNat. exists k.
+        admit.
+          (* exists k. apply redd_to_conv in A1_red_nat as A1_conv_nat. 
+          split; eauto 7 using sim_left_redd, sim_sym, redd_conv, conv_sym. *)
+    - admit.
+    (* - intros. split; intros.
+        + apply LR_U; eauto using sim_left_redd, sim_sym.
+        + rewrite H0 in *. destruct H3 as (R' & lr). destruct (H t u R' lr).
+          apply redd_to_conv in A1_red_U as A1_conv_U.
+          exists R'. eapply H3; eauto using sim_conv, conv_sym. *)
+    - intros. split; intros.
+        + eapply sim_left_redd_whnf in A1_red_pi as (_pi & A'_redd_pi & pi_sim); eauto.
+          eapply aconv_inv in pi_sim. simpl in pi_sim. subst.
+          eapply sim_left_redd_whnf in A2_red_pi as (_pi & B'_redd_pi & pi_sim); eauto.
+          eapply aconv_inv in pi_sim. simpl in pi_sim. subst.
+          eapply LR_pi; eauto 6 using sim_left_redd, sim_sym, sim_to_conv, conv_trans, conv_sym.
+        + rewrite H in *. destruct H4. apply redd_whnf_to_conv in A1_red_pi as A1_conv_pi. split.
+            ++ eauto 8 using sim_to_conv, conv_trans, conv_sym, conv_conv.
+            ++ intros.
+               destruct (H1 s1 s2 ϵs). 
+               destruct (LR_escape _ _ _ _ (LR_T s1 s2 ϵs)) as (T1_s1_conv_T2_s2 & K). 
+               destruct (LR_escape _ _ _ _ LR_S). apply H9 in ϵs as s1_conv_s2.
+               apply validity_conv_left in s1_conv_s2 as s1_Wt. 
+               apply validity_conv_right in s1_conv_s2 as s2_Wt.
+               eapply type_conv in s2_Wt; eauto.
+               eapply H7; eauto.
+               eapply redd_whnf_to_conv in A2_red_pi as pi2.
+               eapply validity_conv_right in pi2. 
+               eapply type_inv_pi in pi2 as (S2_Wt & T2_Wt). 
+                eapply redd_whnf_to_conv in A1_red_pi as pi1.
+               eapply validity_conv_right in pi1. 
+               eapply type_inv_pi in pi1 as (S1_Wt & T1_Wt).
+               eapply aconv_app; eauto using validity_conv_left, refl_ty.
+               eapply aconv_conv; eauto.
+               admit. 
 Admitted.
 
-           
-Lemma LR_irrel l A B1 B2 R1 R2 : 
-    LR l A B1 R1 -> 
-    LR l A B2 R2 -> 
+
+Definition LR_inv_type l A1 A2 A1' R (A1_redd_A1' : ∙ ⊢< Ax l > A1 -->>! A1' : Sort l) : Prop :=
+    match l, A1' with 
+    | prop, _ => LRΩ A1 A2 R
+    | _, Nat => 
+        l = ty 0 /\ 
+        ∙ ⊢< Ax (ty 0) > A1 -->>! Nat : Sort (ty 0) /\ 
+        ∙ ⊢< Ax (ty 0) > A2 -->>! Nat : Sort (ty 0) /\ 
+        R <~> ϵNat
+    | _, Sort l' => 
+        l = Ax l' /\ 
+        ∙ ⊢< Ax (Ax l') > A1 -->>! Sort l' : Sort (Ax l') /\ 
+        ∙ ⊢< Ax (Ax l') > A2 -->>! Sort l' : Sort (Ax l') /\ 
+        R <~> (fun B1 B2 => exists R', LR l' B1 B2 R')
+    | _, Pi i (ty k) S1 T1 => exists S2 T2 ϵS ϵT,
+        l = Ru i (ty k) /\ 
+        ∙ ⊢< Ax (Ru i (ty k)) > A1 -->>! Pi i (ty k) S1 T1 : Sort (Ru i (ty k)) /\
+        ∙ ⊢< Ax (Ru i (ty k)) > A2 -->>! Pi i (ty k) S2 T2 : Sort (Ru i (ty k)) /\
+        ∙ ⊢< Ax i > S1 ≡ S2 : Sort i /\
+        ∙ ,, (i, S1) ⊢< Ax (ty k) > T1 ≡ T2 : Sort (ty k) /\
+        LR i S1 S2 ϵS /\
+        (forall s1 s2 (ϵs : ϵS s1 s2), LR (ty k) (T1 <[ s1 ..]) (T2 <[ s2 ..]) (ϵT s1 s2 ϵs)) /\
+        R <~> ϵPi i (ty k) S1 S2 ϵS T1 T2 ϵT
+    | _, _ => True
+    end.
+
+Lemma LR_inv {l A1 A2 A1' R} (A1_redd_A1' : ∙ ⊢< Ax l > A1 -->>! A1' : Sort l) : LR l A1 A2 R -> LR_inv_type l A1 A2 A1' R A1_redd_A1'.
+Proof.
+    intro lr. generalize l A1 A2 R lr A1' A1_redd_A1'. clear l A1 A2 R lr A1' A1_redd_A1'.
+    refine (LR_ind _ _ _ _ _).
+    - intros. auto. 
+    - intros. 
+      eapply redd_whnf_det in A1_red_nat as A1'_eq_Nat; eauto. subst.
+      simpl. eauto.
+    - intros.
+      eapply redd_whnf_det in A1_red_U as A1'_eq_U; eauto. subst.
+      simpl. eauto.
+    - intros. 
+      eapply redd_whnf_det in A1_red_pi as A1'_eq_pi; eauto. subst.
+      simpl. do 4 eexists. 
+      split; eauto.
+      split; eauto. split; eauto.
+Qed.
+
+Lemma LR_irrel l A B B' R1 R2 : 
+    LR l A B R1 -> 
+    LR l A B' R2 -> 
     forall t1 t2, R1 t1 t2 <-> R2 t1 t2.
 Proof.
+    intro lr1. generalize l A B R1 lr1 B' R2. clear l A B R1 lr1 B' R2.
+    refine (LR_ind _ _ _ _ _).
+    - intros. rewrite LR_prop_eq in H. destruct p, H. destruct (H1 t1 t2), (H2 t1 t2). split; eauto.
+    - intros. eapply (LR_inv A1_red_nat) in H0. destruct H0 as (_ & _ & _ & H0). symmetry. rewrite H. auto.
+    - intros. eapply (LR_inv A1_red_U) in H1. destruct H1 as (_ & _ & _ & H'). rewrite H0. rewrite H'. split; eauto.
+    - intros. eapply (LR_inv A1_red_pi) in H2. 
+      destruct H2 as (S2' & T2' & ϵS' & ϵT' & l_eq & A1_red' & A2_red' & S_eq & T_eq & LR_S' & LR_T' & R_eq).
+      assert (ϵS <~> ϵS') by eauto. rewrite R_eq. 
+      intros. split. 
+      intro.
+      unfold ϵPi. rewrite H in H3. destruct H3. split; auto.
+      intros. assert (forall s1 s2 ϵs, ϵT s1 s2 (proj2 (H2 s1 s2) ϵs) <~> ϵT' s1 s2 ϵs).
+      intros. eapply H1. eauto. 
+      apply H5.
+      assert (ϵT s1 s2 (proj2 (H2 s1 s2) ϵs) (app i (ty k) S1 T1 t1 s1) (app i (ty k) S2 T2 t2 s2)).
+      apply H4.
+      destruct (LR_erasure _ _ _ _ (LR_T s1 s2 (proj2 (H2 s1 s2) ϵs))).
+      eapply H8; eauto. admit. admit. 
+      intro. rewrite H.
+      unfold ϵPi. destruct H3. split; auto.
+      intros. assert (forall s1 s2 ϵs, ϵT s1 s2 ϵs <~> ϵT' s1 s2 (proj1 (H2 s1 s2) ϵs)).
+      intros. eapply H1. eauto. 
+      apply H5.
+      assert (ϵT' s1 s2 (proj1 (H2 s1 s2) ϵs) (app i (ty k) S1 T1 t1 s1) (app i (ty k) S2' T2' t2 s2)).
+      apply H4.
+      destruct (LR_erasure _ _ _ _ (LR_T' s1 s2 (proj1 (H2 s1 s2) ϵs))).
+      eapply H8; eauto. admit. admit.
+Admitted.
+
+
+Definition PER {A} (R:A -> A -> Prop) := 
+    (forall t u, R t u -> R u t) /\ (forall t u v, R t v -> R v u -> R t u).
+
+Lemma PER_refl {A} {R : A -> A -> Prop} {t u} : PER R -> R t u -> R t t.
+Proof.
+    intros. destruct H. eapply H1; eauto.
+Qed.
+
+Lemma LR_iff_rel l A B R R' :
+    R <~> R' ->
+    LR l A B R -> 
+    LR l A B R'.
+Proof.
+    intros. generalize l A B R H0 R' H. clear l A B R H0 R' H. 
+    refine (LR_ind _ _ _ _ _); intros.
+    - rewrite LR_prop_eq. destruct p. split; eauto. intros. rewrite <- H. eauto.
+    - eapply LR_nat; eauto. intros. rewrite <- H0. eauto.
+    - eapply LR_U; eauto. intros. rewrite <- H1. eauto.
+    - eapply LR_pi; eauto. intros. rewrite <- H2. eauto.
+Qed. 
+
+
+Lemma aux' l A B R :
+    LR l A B R ->
+    PER R /\
+    LR l B A R /\ 
+    (forall R' C, LR l B C R' -> LR l A C R' /\ R <~> R') /\
+    (forall R' C, LR l C A R' -> LR l C B R' /\ R <~> R').
+Proof.
+    generalize l A B R. clear l A B R.
+    refine (LR_ind _ _ _ _ _).
+    - intros. split. 2:split. 3:split.
+      + destruct p. split; intros; rewrite H0 in *; eauto using conv_sym, conv_trans.
+      + rewrite LR_prop_eq. destruct p. split; eauto using conv_sym. intros. 
+        rewrite (H0 t u). split; intros; eauto using conv_conv, conv_sym.
+      + intros. rewrite LR_prop_eq in *. destruct H, p. split. split; eauto using conv_trans.
+        intros. rewrite (H0 t u). split; intros; eauto using conv_conv, conv_sym.
+        intros. rewrite (H2 t u). rewrite (H0 t u).  split; intros; eauto using conv_conv, conv_sym.
+      + intros. rewrite LR_prop_eq in *. destruct H, p. split. split; eauto using conv_trans.
+        intros. rewrite (H2 t u). rewrite (H0 t u).  split; intros; eauto using conv_conv, conv_sym.
+    - intros. split. 2:split. 3:split.
+      + split; intros; rewrite H in *. 
+        destruct H0 as (k & H1 & H2). eexists. split; eauto.
+        destruct H0 as (k & t_red & v_red). destruct H1 as (k' & v_red' & u_red).
+        exists k. split. eauto. admit.
+      + eapply LR_nat; eauto.
+      + intros. unshelve eapply LR_inv in H0. shelve. eapply A2_red_nat. 
+        destruct H0 as (_ & _ & C_red & R'_iff_nat). 
+        split. eauto using LR_nat. intros. rewrite H. rewrite R'_iff_nat. split; auto.
+      + intros. admit.
+    - intros. split. 2:split. 3:split.
+      + split; intros; rewrite H0 in *. destruct H1. destruct (H _ _ _ H1) as (_ & H' & _). eexists. eauto.
+        destruct H1. destruct H2. destruct (H _ _ _ H1) as (_ & _  & H' & H'').
+        destruct (H' _ _ H2). eexists. eauto.
+      + eapply LR_U; eauto. 
+      + intros. pose proof H1 as H1'. unshelve eapply LR_inv in H1. shelve. eauto. destruct H1 as (_ & _ & C_red & H').
+        split. eapply LR_U; eauto.
+        intros; split; rewrite H'; rewrite H0; intros; eauto.
+      + admit.
+    - intros. 
+      destruct H0 as (PER_ϵS & LR_S_sym & LR_S_trans_left & LR_S_trans_right).
+      pose proof PER_ϵS as PER_ϵS'.
+      destruct PER_ϵS as (ϵS_sym & ϵS_trans). rename PER_ϵS' into PER_ϵS.
+      assert (forall s1 s2 ϵs, 
+        ϵT s1 s2 ϵs <~> ϵT s2 s1 (ϵS_sym _ _ ϵs) /\ ϵT s1 s2 ϵs <~> ϵT s2 s2 (PER_refl PER_ϵS (ϵS_sym _ _ ϵs))).
+      { intros. pose (ϵs' := ϵS_sym _ _ ϵs). pose (ϵs'' := PER_refl PER_ϵS ϵs').
+        pose (LR_T_s1_s2 := LR_T _ _ ϵs).
+        pose (LR_T_s2_s1 := LR_T _ _ ϵs').
+        pose (LR_T_s2_s2 := LR_T _ _ ϵs'').
+        destruct (H1 _ _ ϵs) as (_ & LR_T_s1_s2' & _).
+        destruct (H1 _ _ ϵs') as (_ & LR_T_s2_s1' & _).
+        destruct (H1 _ _ ϵs'') as (_ & _ & LR_T_trans_left & LR_T_trans_right).
+        eapply LR_T_trans_left in LR_T_s1_s2' as (_ & HA).
+        eapply LR_T_trans_right in LR_T_s2_s1' as (_ & HB).
+        unfold ϵs' in HB.
+        split.
+        + split; intros; rewrite <- HA in *; rewrite <- HB in *; eauto.
+        + unfold ϵs'', ϵs' in *. symmetry. rewrite HA. split; intros; eauto. }
+      split. 2:split. 3:split.
+      + split; intros; rewrite H in *. 
+        ++ destruct H2. split; eauto using conv_sym.
+           intros. destruct (H1 _ _ ϵs) as ((ϵT_sym & ϵT_trans) & _). eapply ϵT_sym.
+           eapply (proj1 (H0 _ _ _)). pose (H3' := H3 _ _ (ϵS_sym _ _ ϵs)). admit.
+        ++ destruct H2, H3. split; eauto using conv_trans.
+           intros. destruct (H1 _ _ ϵs) as ((ϵT_sym & ϵT_trans) & _). eapply ϵT_trans.
+           eapply H4. eapply (proj2 (H0 _ _ _)). pose (H5' := H5 _ _ (PER_refl PER_ϵS (ϵS_sym s1 s2 ϵs))). admit.
+      + eapply LR_pi; eauto using conv_sym, conv_ty_in_ctx_conv. intros.
+        destruct (H1 _ _ (ϵS_sym _ _ ϵs)) as (_ & H3' & _).
+        eapply LR_iff_rel. eapply (proj1 (H0 _ _ _)). eapply H3'.
+        split; intros; rewrite H in *. destruct H2. split. admit.
+        intros. pose (H3' := H3 _ _ (ϵS_sym s2 s1 (ϵS_sym s1 s2 ϵs))). admit.
+        destruct H2. split. admit.
+        intros. pose (H3' := H3 _ _ ϵs). admit.
+      + intros. pose proof H2 as H2'. unshelve eapply LR_inv in H2. shelve. eauto. 
+        destruct H2 as (S' & T' & ϵS' & ϵT' & _ & _ & C_red & S2_eq_S' & T2_eq_T' & LR_S' & LR_T' & R'_iff).
+        pose proof (ϵS_iff_ϵS' := LR_irrel _ _ _ _ _ _ LR_S_sym LR_S').
+        assert (forall s1 s2, ϵS' s1 s2 -> ϵS' s2 s1) as ϵS'_sym. intros. rewrite <- ϵS_iff_ϵS' in *. eauto.
+        (* eassert (∀ (s1 s2 : term) (ϵs : ϵS' s1 s2), LR (ty k) (T1 <[ s1..]) (T' <[ s2..]) _).
+        intros. *)
+
+        (* apply ϵS_sym in ϵs as ϵs'. *)
+        eassert (forall s1 s2 (ϵs : ϵS s1 s2), LR (ty k) (T2 <[ s2..]) (T' <[ s1..]) (ϵT' s2 s1 _)). 
+        intros. pose (ϵs' := proj1 (ϵS_iff_ϵS' _ _) (ϵS_sym _ _ ϵs)).  eapply (LR_T' _ _ ϵs').
+        (* epose proof (ϵT_iff_ϵT' := fun s1 s2 (ϵs : ϵS s1 s2) => LR_irrel _ _ _ _ _ _ (proj1 (proj2 (H1 _ _ ϵs))) _. 
+        shelve. shelve. eapply (LR_T'  _ _ (ϵ)
+        assert (ϵS <~> ϵS'). split;  *)
+        assert (forall s1 s2 ϵs, ϵT s1 s2 ϵs <~> ϵT' s1 s2 (proj1 (ϵS_iff_ϵS' _ _) ϵs)) as ϵT_iff_ϵT'.
+        intros. destruct (H1 _ _ (ϵS_sym _ _ ϵs)) as (_ & K & _).
+        pose (ϵs' := proj1 (ϵS_iff_ϵS' _ _) ϵs).
+        pose (K' := LR_T' _ _ ϵs'). pose proof (L := LR_irrel _ _ _ _ _ _ K K').
+        destruct (H0 _ _ ϵs) as (L' & _). rewrite L'. rewrite L. unfold ϵs'. split; eauto. 
+
+        split.
+        ++ eapply (LR_pi _ _ _ _ _ _ ϵS' _ _ ϵT'); eauto using conv_trans, conv_sym, conv_ty_in_ctx_conv. 
+           eapply LR_S_trans_left in LR_S' as (S1_eq_S' & _). eauto. 
+           intros. pose proof (ϵs' := proj2 (ϵS_iff_ϵS' s1 s2) ϵs).
+           eapply ϵS_sym in ϵs' as ϵs''. 
+           eapply PER_refl in ϵs''.
+           rewrite ϵS_iff_ϵS' in ϵs''.
+           pose (LR_T'' := LR_T' _ _ ϵs'').
+           destruct (H1 _ _ ϵs') as (K & K1 & K2 & K3).
+           unshelve eapply (proj1 (K2 _ _ _)). 2:eauto.
+           eapply LR_iff_rel. 2: apply LR_T''. admit.
+           intros; split; intros; rewrite R'_iff in *.
+           destruct H3. split. admit. 
+           intros. pose (H4' := H4 _ _ ϵs). admit.
+           destruct H3. split. admit.
+           intros. pose (H4' := H4 _ _ ϵs). admit.
+        ++ intros; split; intro; rewrite H in *; rewrite R'_iff in *.
+           destruct H3. split. admit.
+           intros. pose (H4' := H4 _ _ (proj2 (ϵS_iff_ϵS' _ _) ϵs)). rewrite ϵT_iff_ϵT' in *. admit.
+           destruct H3. split. admit.
+           intros. pose (H4' := H4 _ _ (proj1 (ϵS_iff_ϵS' _ _) ϵs)). rewrite ϵT_iff_ϵT' in *. admit.
+      + admit.
+Admitted.
+           
+
+Definition TmLR l t u A := exists B R, LR l A B R /\ R t u.
+
+Notation "⊩< l > t ≡ u : A" := (TmLR l t u A) (at level 50, t, u, A at next level).
+
+
+Lemma LR_conv l A B t u R : 
+    LR l A B R -> TmLR l t u A -> TmLR l t u B.
+Proof.
+    intros. destruct H0 as (B' & R' & LR & R'_t_u).
+    eapply LR_irrel in R'_t_u as R_t_u. 2: apply H. 2:eauto.
+    exists A. exists R. split; auto. admit.
 Admitted.
 
 
